agda itree wacky development

MinHS/min-minhs.hs
@@ -1,0 +1,121 @@
+--
+-- interpreter examples: assume types are checked
+-- f $ a b c.... means f (a b c...)
+--
+
+data Expr =
+    Num Int
+  | Lit Bool
+  | If Expr Expr Expr
+  | Apply Expr Expr
+  | Plus Expr Expr
+  | Eq Expr Expr
+  -- note: HOAS used here, use haskell closures to avoid substitution issues
+  | Recfun (Expr -> Expr -> Expr)
+
+--
+-- by-name: substitute directly during an apply, don't eval argument x
+-- function values store unevaluated expressions
+--
+data Val = BV Bool | IV Int | FV (Expr -> Expr -> Expr)
+instance Show Val where
+  show (BV b) = show b
+  show (IV i) = show i
+  show (FV f) = "F"
+
+evalByName :: Expr -> Val
+evalByName (Num i) = IV i
+evalByName (Lit b) = BV b
+evalByName (If v l r) = case evalByName v of
+    BV b -> if b then evalByName l else evalByName r
+    _ -> undefined
+evalByName (Plus x y) = case (evalByName x,evalByName y) of
+  (IV x',IV y') -> IV $ x' + y'
+  _ -> undefined
+evalByName (Eq x y) = case (evalByName x,evalByName y) of
+  (IV x',IV y') -> BV $ x' == y'
+  (BV x', BV y') -> BV $ x' == y'
+  _ -> undefined
+-- important cases!
+evalByName (Recfun f) = FV f 
+evalByName (Apply f x) =
+  case evalByName f of
+    FV f' -> evalByName $ f' f x
+    _ -> undefined
+
+--
+-- by-value: eval argument first before applying function
+--
+data Value = B Bool | I Int | F (Value -> Value)
+instance Show Value where
+  show (B b) = show b
+  show (I i) = show i
+  show (F f) = show "F"
+
+val_to_expr :: Value -> Expr
+val_to_expr (I i) = Num i
+val_to_expr (B b) = Lit b
+val_to_expr (F f) = Recfun $ \g x -> val_to_expr $ f (evalByVal x)
+
+evalByVal :: Expr -> Value
+evalByVal (Num i) = I i
+evalByVal (Lit b) = B b
+evalByVal (If v l r) = case evalByVal v of
+    B b -> if b then evalByVal l else evalByVal r
+    _ -> undefined
+evalByVal (Plus x y) = case (evalByVal x,evalByVal y) of
+  (I x',I y') -> I $ x' + y'
+  _ -> undefined
+evalByVal (Eq x y) = case (evalByVal x,evalByVal y) of
+  (I x',I y') -> B $ x' == y'
+  (B x', B y') -> B $ x' == y'
+  _ -> undefined
+-- important cases!
+evalByVal (Recfun f) = F $ \x -> evalByVal (f (Recfun f) (val_to_expr x))
+evalByVal (Apply f x) =
+  case evalByVal f of
+    F f' -> f' $ evalByVal x
+    _ -> undefined
+
+--
+-- examples
+--
+
+-- cheeky metalanguage shortcuts
+eq0 x = (Eq x (Num 0))
+minus1 x = Plus x (Num (-1))
+
+-- we do manual currying to express products
+prod :: Expr
+prod = Recfun $ \g n ->
+  Recfun $ \f x ->
+  If (eq0 x)
+  (Num 0) $
+  Plus n (Apply f (minus1 x))
+
+-- try: evalByName (Apply fact (Num 9))
+-- try: evalByVal  (Apply fact (Num 9))
+-- note the difference in speed!
+-- why?! If you can explain why this happens you're good to go for as1 ;)
+fact' :: Expr
+fact' = 
+  Recfun $ \f n ->
+  Recfun $ \_ accum ->
+  If (eq0 n)
+  accum
+  (Apply (Apply f (minus1 n)) (Apply (Apply prod accum) n))
+
+fact :: Expr
+fact = Recfun $ \_ n -> Apply (Apply fact' n) (Num 1) 
+
+-- higher order functions test
+ide :: Expr
+ide = Recfun $ \self x -> x
+
+idm :: Expr
+idm = Recfun $ \self x-> If (Eq x (Num 0))
+  ide $
+  Apply self (Plus x (Num (-1)))
+
+comp :: Expr
+comp = Recfun $ \_ f -> Recfun $ \_ g -> Recfun $ \_ x -> Apply f (Apply g x)
