agda/itree.agda
@@ -1,30 +1,57 @@
 {-# OPTIONS --copatterns --guardedness #-}
 
-open import Agda.Primitive
-
-data ℕ : Set where
-  zero : ℕ
-  suc : ℕ → ℕ
-{-# BUILTIN NATURAL ℕ #-}
-
-data 𝟙 : Set where
-  ⋆ : 𝟙
+open import Function.Base using (case_of_; case_return_of_)
+open import logic
+open import eq
 
 mutual
   data itree-ind (E : Set → Set) (A R : Set) : Set₁ where
-    Ret : R → itree-ind E A R
-    Tau : Itree E A R → itree-ind E A R
-    Vis : (A → Itree E A R) → itree-ind E A R
+    ret : R → itree-ind E A R
+    tau : Itree E A R → itree-ind E A R
+    vis : E A → (A → Itree E A R) → itree-ind E A R
 
   record Itree (E : Set → Set) (A R : Set) : Set₁ where
     coinductive
     field
       alg : itree-ind E A R
 
-data IO : Set → Set where
-  input : IO ℕ
-  output : ℕ → IO 𝟙
+open Itree
 
-mutual
-  spin : Itree (λ x → 𝟙) 𝟙 𝟙
-  Itree.alg spin = Tau spin
+Ret : {E : Set → Set} {A R : Set} → R → Itree E A R
+alg (Ret r) = ret r
+
+Tau : {E : Set → Set} {A R : Set} → Itree E A R → Itree E A R
+alg (Tau t) = tau t
+
+Vis : {E : Set → Set} {A R : Set} → E A → (A → Itree E A R) → Itree E A R
+alg (Vis e k) = vis e k
+
+trigger : {E : Set → Set} {A : Set} (e : E A) → Itree E A A
+trigger e = Vis e (λ x → Ret x)
+
+-- algebra (Itree E A R) × ktree
+-- (Ret r,   k).ret = ???
+-- (Tau t,   k).tau = (t,k)
+-- (Vis e g, k).vis = vis e λx.((g x),k) A -> X --bind ∘-> A -> Y
+bind : {E : Set → Set} {A R S : Set}
+     → Itree E A R → (R → itree-ind E A S)
+     → Itree E A S
+alg (bind t k) with alg t
+...            | ret r = (k r)
+...            | tau t = tau (bind t k)
+...            | vis e g = vis e (λ x → bind (g x) k)
+
+iter : {E : Set → Set} {A B R : Set}
+     → (A → Itree E A (A ＋ B))
+     → A → Itree E A B
+alg (iter body a) = alg (bind (body a)
+                         λ { (inl a) → tau (iter body a)
+                           ; (inr b) → ret b
+                         }
+                    )
+
+-- spin
+spin : Itree (λ x → 𝟙) 𝟙 𝟙
+alg spin = tau spin
+
+-- TODO need bisimulation as setoid equivalence for everything
